README.md
@@ -8,3 +8,4 @@ Unsolved:
 - SLF:
  + Equiv.v: not_congr, optimize_0plus
  + Hoare2.v: improve_dcom, implement_dcom
+ + Smallstep.v: compiler_is_correct
